theories/equivalence/StringUtils.v
@@ -7,12 +7,25 @@ From Stdlib Require Import Lia.
 Import ListNotations.
 
 
-Fixpoint get_max_label_str (l : StringLang.program) : nat :=
+Fixpoint get_max_label (l : StringLang.program) : nat :=
   match l with
   | [] => 0
   | StringLang.Instr opt_lbl _ :: t =>
       match opt_lbl with
-      | None => get_max_label_str t
-      | Some (A n) => Nat.max n (get_max_label_str t)
+      | None => get_max_label t
+      | Some (A n) => Nat.max n (get_max_label t)
       end
+  end.
+
+
+
+Fixpoint label_in_instr p_str (lbl : label)  :=
+  match p_str with
+  | [] => false
+  | StringLang.Instr opt_lbl _ :: t => match opt_lbl with 
+                                       | Some lbl' => if eqb_lbl lbl lbl'
+                                                      then true
+                                                      else label_in_instr t lbl
+                                       | None => label_in_instr t lbl
+                                       end
   end.
