theories/nat_lang/NatLang.v
@@ -49,7 +49,7 @@ From Triq Require Export LanguagesCommon.
 Inductive statement : Type :=
   | INCR : variable -> statement
   | DECR : variable -> statement
-  | IF_GOTO   : variable -> option label -> statement.
+  | IF_GOTO   : variable -> label -> statement.
 
 
 Inductive instruction : Type :=
@@ -135,20 +135,19 @@ Definition create_state x :=
 
 
 Definition eq_inst_label (instr : instruction ) (opt_lbl : option label) :=
-  match instr, opt_lbl with 
-  | Instr (Some lbl_a) _, Some lbl_b => eqb_lbl lbl_a lbl_b
-  | _, _                => false
+  match instr with 
+  | Instr opt_lbl' _ => eqb_opt_lbl opt_lbl' opt_lbl
   end.
 
 (** Função para encontrar a posição da primeira instrução com certa label 
     em um programa *)
 
 
-Fixpoint get_labeled_instr (p : list instruction) (lbl : option label) : nat :=
+Fixpoint get_labeled_instr (p : list instruction) (lbl : label) : nat :=
   match p with
   | [] => 0
   | h :: t =>
-      if eq_inst_label h lbl
+      if eq_inst_label h (Some lbl)
       then 0
       else 1 + get_labeled_instr t lbl
   end.
